theories/Notations.v
@@ -16,7 +16,7 @@ Open Scope typing_scope.
 Class WfContext (ta : tag) := wf_context : context -> Set.
 Class WfType (ta : tag) := wf_type : context -> term -> Set.
 Class Typing (ta : tag) := typing : context -> term -> term -> Set.
-Class Infering (ta : tag) := infering : context -> term -> term -> Set.
+Class Inferring (ta : tag) := inferring : context -> term -> term -> Set.
 Class ConvType (ta : tag) := conv_type : context -> term -> term -> Set.
 Class ConvTerm (ta : tag) := conv_term : context -> term -> term -> term -> Set.
 Class ConvNeu (ta : tag) := conv_neu : context -> term -> term -> term -> Set.
@@ -37,13 +37,15 @@ Notation "[ Γ |- t : A ]" := (typing Γ A t)
 Notation "[ Γ |-[ ta  ] t : A ]" :=
   (typing (ta := ta) Γ A t) (at level 0, ta, Γ, t, A at level 50) : typing_scope.
 (* The term t infers A in Γ *)
-Notation "[ Γ |- t ▹ A ]" := (infering Γ A t)
+Notation "[ Γ |- t ▹ A ]" := (inferring Γ A t)
   (at level 0, Γ, t, A at level 50, only parsing) : typing_scope.
 Notation "[ Γ |-[ ta  ] t ▹ A ]" :=
-  (infering (ta := ta) Γ A t) (at level 0, ta, Γ, t, A at level 50) : typing_scope.
+  (inferring (ta := ta) Γ A t) (at level 0, ta, Γ, t, A at level 50) : typing_scope.
 (* The term t infers the reduced A in Γ *)
 Reserved Notation "[ Γ |- t ▹h A ]" (at level 0, Γ, t, A at level 50).
 Reserved Notation "[ Γ |-[ ta  ] t ▹h A ]" (at level 0, ta, Γ, t, A at level 50).
+(* The term t checks against A in Γ *)
+Reserved Notation "[ Γ |- t ◃ A ]" (at level 0, Γ, t, A at level 50).
 (* Types A and B are convertible in Γ *)
 Notation "[ Γ |- A ≅ B ]" := (conv_type Γ A B)
   (at level 0, Γ, A, B at level 50, only parsing) : typing_scope.
