theories/AlgorithmicTyping.v
@@ -9,9 +9,9 @@ Section Definitions.
   Close Scope typing_scope.
 
   Inductive WfTypeAlg : context -> term -> Type :=
-    | wfTypeU Γ : [Γ |- U]
+    | wfTypeU Γ : [ Γ |- U ]
     | wfTypeProd {Γ na A B} :
-      [Γ |- A] ->
+      [Γ |- A ] ->
       [Γ,, vass na A |- B] ->
       [Γ |- tProd na A B]
     | wfTypeUniv {Γ A} :
@@ -26,7 +26,7 @@ Section Definitions.
       [Γ ,, (vass na A) |- B ▹h U ] ->
       [ Γ |- tProd na A B ▹ U ]
     | infLam {Γ} {na} {A B t} :
-      [ Γ |- A ] ->
+      [ Γ |- A] ->
       [ Γ ,, vass na A |- t ▹ B ] -> 
       [ Γ |- tLambda na A t ▹ tProd na A B]
     | infApp {Γ} {na} {f a A B} :
@@ -41,7 +41,7 @@ Section Definitions.
   with CheckAlg : context -> term -> term -> Type :=
     | checkConv {Γ t A A'} :
       [ Γ |- t ▹ A ] -> 
-      [ Γ |- A ≅ A' ] -> 
+      [ Γ |- A ≅ A'] -> 
       [ Γ |- t : A' ]
   with ConvTypeAlg : context -> term -> term  -> Type :=
     | typeConvRed {Γ A A' B B'} :
@@ -57,7 +57,7 @@ Section Definitions.
     | typeUnivConvAlg {Γ} :
       [Γ |- U ≅h U]
     | typeNeuConvAlg {Γ M N} :
-      [ Γ |- M ~ N ▹ U ] -> 
+      [ Γ |- M ~h N ▹ U ] -> 
       [ Γ |- M ≅h N]
   with ConvNeuAlg : context -> term -> term  -> term -> Type :=
     | neuVarConvAlg {Γ n decl} :
@@ -111,11 +111,109 @@ Section Definitions.
   and   "[ Γ |- t : T ]" := (CheckAlg Γ T t)
   and   "[ Γ |- A ≅ B ]" := (ConvTypeAlg Γ A B)
   and   "[ Γ |- A ≅h B ]" := (ConvTypeRedAlg Γ A B)
-  and   "[ Γ |- m ~ n ▹ T ]" := (ConvNeuAlg Γ m n T)
-  and   "[ Γ |- m ~h n ▹ T ]" := (ConvNeuRedAlg Γ m n T)
-  and   "[ Γ |- t ≅ u : T ]" := (ConvTermAlg Γ t u T)
-  and   "[ Γ |- t ≅h u : T ]" := (ConvTermRedAlg Γ t u T)
+  and   "[ Γ |- m ~ n ▹ T ]" := (ConvNeuAlg Γ T m n)
+  and   "[ Γ |- m ~h n ▹ T ]" := (ConvNeuRedAlg Γ T m n)
+  and   "[ Γ |- t ≅ u : T ]" := (ConvTermAlg Γ T t u)
+  and   "[ Γ |- t ≅h u : T ]" := (ConvTermRedAlg Γ T t u)
   and   "[ Γ |- t ⇒ t' ]" := (OneRedAlg Γ t t')
   and   "[ Γ |- t ⇒* t' ]" := (RedClosureAlg Γ t t').
 
+  (* Inductive WfContextAlgo : context -> Type :=
+  | conNilAlg : [|- ε]
+  | conConsAlg {Γ na A} :
+    [|- Γ] ->
+    [ Γ |- A] ->
+    [|- Γ,, vass na A]
+  where "[ |- Γ ]" := (WfContextAlgo Γ). *)
+
 End Definitions.
+
+Module AlgorithmicTypingData.
+
+  (* In algorithmic typing, we never check contexts! *)
+  #[export] Instance WfContext_Algo : WfContext al := fun _ => True.
+  #[export] Instance WfType_Algo : WfType al := WfTypeAlg.
+  #[export] Instance Inferring_Algo : Inferring al := InferAlg.
+  #[export] Instance Checking_Algo : Typing al := CheckAlg.
+  #[export] Instance ConvType_Algo : ConvType al := ConvTypeAlg.
+  #[export] Instance ConvTerm_Algo : ConvTerm al := ConvTermAlg.
+  #[export] Instance ConvNeu_Algo : ConvNeu al := ConvNeuAlg.
+  (* Reduction is untyped *)
+  #[export] Instance OneRedType_Algo : OneRedType al := OneRedAlg.
+  #[export] Instance OneRedTerm_Algo : OneRedTerm al :=
+  fun Γ _ t u => OneRedAlg Γ t u.
+
+  Ltac fold_algo :=
+    change WfTypeAlg with wf_type in *;
+    change InferAlg with inferring in * ;
+    change CheckAlg with typing in * ;
+    change ConvTypeAlg with conv_type in * ;
+    change ConvTermAlg with conv_term in * ;
+    change ConvNeuAlg with conv_neu in *.
+
+End AlgorithmicTypingData.
+
+Notation "[ Γ |- t ▹h T ]" := (InferRedAlg Γ T t) : typing_scope.
+Notation "[ Γ |- A ≅h B ]" := (ConvTypeRedAlg Γ A B) : typing_scope.
+Notation "[ Γ |- m ~h n ▹ T ]" := (ConvNeuRedAlg Γ m n T) : typing_scope.
+Notation "[ Γ |- t ≅h u : T ]" := (ConvTermRedAlg Γ t u T) : typing_scope.
+Notation "[ Γ |- t ⇒ t' ]" := (OneRedAlg Γ t t') : typing_scope.
+Notation "[ Γ |- t ⇒* t' ]" := (RedClosureAlg Γ t t') : typing_scope.
+
+Section InductionPrinciples.
+  Import AlgorithmicTypingData.
+
+Scheme 
+    Minimality for WfTypeAlg Sort Type with
+    Minimality for InferAlg Sort Type with
+    Minimality for InferRedAlg Sort Type with
+    Minimality for CheckAlg Sort Type with
+    Minimality for ConvTypeAlg Sort Type with
+    Minimality for ConvTypeRedAlg Sort Type with
+    Minimality for ConvNeuAlg Sort Type with
+    Minimality for ConvNeuRedAlg Sort Type with
+    Minimality for ConvTermAlg Sort Type with
+    Minimality for ConvTermRedAlg Sort Type with
+    Minimality for OneRedAlg Sort Type with
+    Minimality for RedClosureAlg Sort Type.
+
+Combined Scheme _WfAlgoInduction from
+    WfTypeAlg_rect_nodep,
+    InferAlg_rect_nodep,
+    InferRedAlg_rect_nodep,
+    CheckAlg_rect_nodep,
+    ConvTypeAlg_rect_nodep,
+    ConvTypeRedAlg_rect_nodep,
+    ConvNeuAlg_rect_nodep,
+    ConvNeuRedAlg_rect_nodep,
+    ConvTermAlg_rect_nodep,
+    ConvTermRedAlg_rect_nodep,
+    OneRedAlg_rect_nodep,
+    RedClosureAlg_rect_nodep.
+    
+Definition WfAlgoInductionConcl
+  (PTy : context -> term -> Type)
+  (PInf PInfRed PCheck PTyEq PTyRedEq : context -> term -> term -> Type)
+  (PNeEq PNeRedEq PTmEq PTmRedEq : context -> term -> term -> term -> Type)
+  (PORed PCRed : context -> term -> term -> Type) :=
+  (forall (Γ : context) (A : term), [Γ |- A] -> PTy Γ A)
+  × (forall (Γ : context) (A t : term), [Γ |- t ▹ A] -> PInf Γ A t)
+  × (forall (Γ : context) (A t : term), [Γ |- t ▹h  A] -> PInfRed Γ A t)
+  × (forall (Γ : context) (A t : term), [Γ |- t : A] -> PCheck Γ A t)
+	× (forall (Γ : context) (A B : term), [Γ |- A ≅ B] -> PTyEq Γ A B)
+  × (forall (Γ : context) (A B : term), [Γ |- A ≅h B] -> PTyRedEq Γ A B)
+  × (forall (Γ : context) (A m n : term), [Γ |- m ~ n ▹ A] -> PNeEq Γ A m n)
+  × (forall (Γ : context) (A m n : term), [Γ |- m ~h n ▹ A] -> PNeRedEq Γ A m n)
+  × (forall (Γ : context) (A t u : term), [Γ |- t ≅ u : A] -> PTmEq Γ A t u)
+  × (forall (Γ : context) (A t u : term), [Γ |- t ≅h u : A] -> PTmRedEq Γ A t u)
+  × (forall (Γ : context) (t u : term), [Γ |- t ⇒ u] -> PORed Γ t u)
+  × (forall (Γ : context) (t u : term), [Γ |- t ⇒* u] -> PCRed Γ t u).
+
+Definition WfAlgoInduction :=
+  ltac:(let ind := fresh "ind" in
+      pose (ind := _WfAlgoInduction);
+      fold_algo ;
+      let ind_ty := type of ind in
+      exact (ind : ind_ty)).
+
+End InductionPrinciples.
